argh

aabb.dfy
@@ -1,6 +1,11 @@
 datatype AABB = AABB(min_x : int, min_y : int, max_x : int, max_y : int)
 datatype InOut = In(idx : int) | Out(idx : int)
 
+predicate before(f : InOut, s : InOut)
+{
+	f.idx == s.idx ==> In(f.idx) == f && Out(f.idx) == s
+}
+
 function overlaps_x (a : AABB, b : AABB) : bool
 {
 	!(a.max_x < b.min_x || b.max_x < a.min_x)
@@ -15,12 +20,18 @@ function overlaps (a : AABB, b : AABB) : bool
 	overlaps_x(a,b) && overlaps_y(a,b)
 }
 
+predicate in_before_out(li : seq<InOut>, k : int)
+{
+	forall i :: 0 <= i < |li| ==> In(k) in li[i..] && In(k) !in li[i + 1..] ==> Out(k) in li[i + 1..]
+}
+
 method order_by_x (li : seq<AABB>) returns (order : seq<InOut>)
 	ensures forall i :: 0 <= i < |li| ==> In(i) in order && Out(i) in order
 	ensures forall i :: 0 <= i < |order| ==> 0 <= order[i].idx < |li|
 	ensures |order| == |li| + |li|
 	ensures |order| % 2 == 0
-	//ensures forall i :: 0 <= i < |order| -1 ==> forall x :: In(x) in order[..i] ==> Out(x) in order[i..]
+	ensures forall i :: 0 <= i < |li| ==> in_before_out(order, i)
+	ensures |multiset(order)| == |order|
 {
 	order := [];
 	for i := 0 to |li|
@@ -29,22 +40,40 @@ method order_by_x (li : seq<AABB>) returns (order : seq<InOut>)
 		invariant |order| == i + i
 		invariant 0 <= i <= |li|
 		invariant |order| % 2 == 0
+		invariant forall j :: 0 <= j < i ==> in_before_out(order, j)
 	{
 		assert 0 <= i < |li|;
 		assert forall m :: 0 <= m < i ==> In(m)  in order;
 		assert forall m :: 0 <= m < i ==> Out(m) in order;
 
-		var in_idx  : int := |order|;
-		var out_idx : int := |order| + 1;
-		order := order + [In(i), Out(i)];
+
+		var in_idx  : int := |order| / 2;
+		var out_idx : int := |order|;
+
+		ghost var old_order : seq<InOut> := order;
+		assert forall j :: 0 <= j < i ==> in_before_out(order, j);
+		order := 
+		    order[..in_idx] 
+		  + [In(i)] 
+		  + order[in_idx..out_idx] 
+		  + [Out(i)] 
+		  + order[out_idx..];
+		assert forall j :: 0 <= j <= i ==> in_before_out(order, j);
+		
+
+		
 
 
 		assert In(i)  == order[ in_idx];
-		assert Out(i) == order[out_idx];
+		assert Out(i) == order[out_idx + 1];
+		assert exists j,k :: 0 <= j < k < |order| && before(order[j], order[k]);
 		assert exists j,k :: 0 <= j < k < |order| && In(i) == order[j] && Out(i) == order[k];
 		assert exists j :: 0 <= j < |order| && In(i)  == order[j];
 		assert exists k :: 0 <= k < |order| && Out(i) == order[k];
 		assert exists j,k :: 0 <= j < k < |order| && In(i) == order[j] && Out(i) == order[k];
+
+		assert exists j,k :: 0 <= j < k < |order| && before(order[j], order[k]);
+
 		
 	}
 }
@@ -53,7 +82,6 @@ method split_along_x(li : seq<AABB>) returns (split : bool, f : seq<AABB>, s : s
 	//ensures |li| == |f| + |s|
 	//ensures forall x :: x in f ==> x !in s
 	//ensures forall x :: x in s ==> x !in f
-	//ensures |f| + |s| == |li|
 {
 	split := false;
 	f := li;
@@ -62,9 +90,9 @@ method split_along_x(li : seq<AABB>) returns (split : bool, f : seq<AABB>, s : s
 	{
 		return;
 	}else{
-		split := true;
 		var order : seq<InOut> := order_by_x(li);
 		assert |order| == |li| + |li|;
+		
 		var in_count    : int := 0;
 		var out_count : int := 0;
 		var split_idx : int := 0;
@@ -84,6 +112,7 @@ method split_along_x(li : seq<AABB>) returns (split : bool, f : seq<AABB>, s : s
 				break;
 			}
 		}
+		split := split_idx != |order|;
 		assert 0 <= split_idx <= |order|;
 		//assert split_idx % 2 == 0;
 
@@ -93,20 +122,34 @@ method split_along_x(li : seq<AABB>) returns (split : bool, f : seq<AABB>, s : s
 		var second_order : seq<InOut> := order[split_idx..];
 
 		//assert forall i :: In(i) in first_order ==> Out(i) in first_order;
+		ghost var total : int := 0;
 		f := [];
 		for i := 0 to |first_order|
+			invariant total == |f|
 		{
+
 			match first_order[i]
-			case In(idx) => f := f + [li[idx]];
+			case In(idx) => 
+			{
+				f := f + [li[idx]];
+				total := total + 1;
+			}
 			case Out(_)  => {}
 		}
 		s := [];
 		for i := 0 to |second_order|
+			invariant total == |f| + |s|
 		{
 			match second_order[i]
-			case In(idx) => s := s + [li[idx]];
+			case In(idx) =>
+			{
+				s := s + [li[idx]];
+				total := total + 1;
+			}
 			case Out(_)  => {}
 		}
+		assert total == |f| + |s|;
+		//assert total == |li|;
 		return;
 	}
 }
@@ -141,13 +184,15 @@ method partition_AABBs(li : seq<AABB>) returns (clusters : seq<seq<AABB>>)
 	assert 0 <= |li| - |clusters|;
 
 	while true
-		//invariant 0 <= |li| - |clusters| 
+		//invariant |clusters| <= |li| 
 		//decreases |li| - |clusters|
 		decreases *
 	{
 		ghost var before : seq<seq<AABB>> := clusters;
 		var added : int := 0;
+
 		for c := 0 to |clusters|
+			//invariant |clusters| <= |li| 
 			invariant 0 <= c <= |clusters|
 			invariant |clusters| >= |before|
 			invariant |before| + added == |clusters|
